\documentclass{article}
\usepackage{graphicx}
\usepackage{amsmath} 
\usepackage{pgfplots}
\usepackage{adjustbox}
\usepackage{subcaption}

\title{Linear Regression}
\begin{document}
  \pagenumbering{gobble}
  \maketitle
  \newpage
  \pagenumbering{arabic}

\section*{Linear Regression}
We have to arrays of numbers $X$ and $Y$. Array $X$ contains independent data points. Array $Y$ contains dependent data points $y_i,i=1,â€¦,m$.

We want to find $\hat{y}(x)$, that accurately represents given data.\\

\section*{Assumptions}

\begin{itemize}
\item Linear relationship
\item Little or no multi-collinearity
\item Little or no auto-correlation
\item Homoscedasticity
\end{itemize}

\section*{Least Squares Regression}

Total squared error is defined as: 
$$E = \sum_{i=1}^m (\hat{y} - y_i)^2$$. 

The individual errors or residuals are defined as: 
$$e_i = (\hat{y} - y_i)$$.

We try to minimize total squared error and $E = \|{e}\|_{2}^{2}$.

\section*{Derivation}

Estimation $\hat{y}(x_i)$ for each point $x_i$:

$$\hat{y}(x_1) = {\alpha}_1 f_1(x_1) + {\alpha}_2 f_2(x_1) + \cdots + {\alpha}_n f_n(x_1),$$
$$\hat{y}(x_2) = {\alpha}_1 f_1(x_2) + {\alpha}_2 f_2(x_2) + \cdots + {\alpha}_n f_n(x_2),$$
\begin{center}$ \cdots $ \end{center}
$$\hat{y}(x_m) = {\alpha}_1 f_1(x_m) + {\alpha}_2 f_2(x_m) + \cdots + {\alpha}_n f_n(x_m)$$

We can write this system of equations in terms of column vectors $\hat{Y}$ and $\beta$:\\

$\hat{Y}_i = \hat{y}(x_i)$\\
$\beta_i = {\alpha}_i$\\

and $m x n$ matrix $A$ such that it's i-th column equals $F_i(x)$.\\

The system of equations becomes then: $\hat{Y} = A{\beta}$\\

The total squared error is given by E:

$$E = \|{\hat{Y} - Y}\|_{2}^2$$

$\hat{Y}$, that is closest to $Y$ is the one that can point perpendicularly to $Y$ .

$${\text{dot}}(\hat{Y}, Y - \hat{Y}) = 0$$

$$\hat{Y}^T (Y - \hat{Y}) = 0$$

$$(A{\beta})^T(Y - A{\beta}) = 0$$

$${\beta}^T A^T Y - {\beta}^T A^T A {\beta} = {\beta}^T(A^T Y - A^T A {\beta}) = 0$$

$$A^T Y - A^T A {\beta} = 0$$\\

We arrive at the least squares regression formula:

$${\beta} = (A^T A)^{-1} A^T Y$$


\end{document}